Classical_Extra.thy
@@ -90,14 +90,6 @@ proof (unfold register_def, intro conjI allI)
     by (auto simp: permutation_register_def)
 qed
 
-lemma register_prod1: \<open>register (\<lambda>a. rel_prod a Id)\<close>
-  unfolding register_def apply (intro conjI allI)
-  using update_2hom_left_is_hom tensor_update_is_2hom apply blast
-    apply (simp add: tensor_update_mult)
-   apply simp
-  by (simp add: rel_prod_converse)
-
-
 definition register_from_setter :: \<open>('b\<Rightarrow>'a) \<Rightarrow> ('a\<Rightarrow>'b\<Rightarrow>'b) \<Rightarrow> ('a,'b) preregister\<close> where
   \<open>register_from_setter g s a = {(s ax b, s ay b) | b ax ay. (ax,ay) \<in> a}\<close>
 
